<?xml version="1.0"?>
<!--
  union of
  RDF Schema declaration Draft for the Qualified Dublin Core Element Set 2002/05/15
  RDF Schema declaration Draft for DCMI Type Vocabulary 2002/05/15
-->
<!DOCTYPE rdf:RDF [
  <!ENTITY rdfns 'http://www.w3.org/1999/02/22-rdf-syntax-ns#'>
  <!ENTITY rdfsns 'http://www.w3.org/2000/01/rdf-schema#'>
  <!ENTITY dcns 'http://purl.org/dc/elements/1.1/'>
  <!ENTITY dctermsns 'http://purl.org/dc/terms/'>
  <!ENTITY dctypens 'http://purl.org/dc/dcmitype/'>
]>
<rdf:RDF xmlns:rdf="&rdfns;" xmlns:rdfs="&rdfsns;" xmlns:dc="&dcns;" xmlns:dcterms="&dctermsns;" xmlns:dctype="&dctypens;">
  <!-- Description of this Schema -->
  <rdf:Description rdf:about="&dctermsns;">
    <dc:title>The Dublin Core Terms namespace providing access
   to it's content by means of an RDF Schema</dc:title>
    <dc:publisher>The Dublin Core Metadata Initiative</dc:publisher>
    <dc:description>The Dublin Core Terms namespace provides URIs for the
   Dublin Core Element Set Qualifier Vocabulary. Vocabulary terms are
   declared using RDF Schema language to support RDF applications.
   The Dublin Core qualifiers form a richer vocabulary,
   which is intended to facilitate discovery of resources.
  </dc:description>
    <dc:language>English</dc:language>
    <dcterms:requires rdf:resource="http://www.dublincore.org/documents/2000/07/11/dcmes-qualifiers/"/>
    <dc:source rdf:resource="http://www.dublincore.org/documents/2000/07/11/dcmes-qualifiers/"/>
  </rdf:Description>
  <!-- Begin: Title  -->
  <!-- Title refinement declarations  -->
  <rdf:Property rdf:about="&dctermsns;alternative">
    <rdfs:label>Alternative</rdfs:label>
    <rdfs:comment>Any form of the title used as a substitute or
    alternative to the formal title of the resource.</rdfs:comment>
    <rdfs:subPropertyOf rdf:resource="&dcns;title"/>
    <rdfs:isDefinedBy rdf:resource="&dctermsns;"/>
  </rdf:Property>
  <rdf:Description rdf:about="&rdfsns;label">
    <rdfs:subPropertyOf rdf:resource="&dcns;title"/>
  </rdf:Description>
  <!-- End: Title Declaration -->
  <!-- End: Title  -->
  <!-- Begin: Subject  -->
  <!-- Encoding Scheme declarations -->
  <rdfs:Class rdf:about="&dctermsns;SubjectScheme">
    <rdfs:label>Subject Encoding Schemes</rdfs:label>
    <rdfs:comment>A set of subject encoding schemes
    and/or formats</rdfs:comment>
    <rdfs:isDefinedBy rdf:resource="&dctermsns;"/>
  </rdfs:Class>
  <rdfs:Class rdf:about="&dctermsns;LCSH">
    <rdfs:label>LCSH</rdfs:label>
    <rdfs:comment>Library of Congress Subject Headings
  </rdfs:comment>
    <rdf:type rdf:resource="&dctermsns;SubjectScheme"/>
    <rdfs:isDefinedBy rdf:resource="&dctermsns;"/>
  </rdfs:Class>
  <rdfs:Class rdf:about="&dctermsns;LCC">
    <rdfs:label>LCC</rdfs:label>
    <rdfs:comment>Library of Congress Classification
  </rdfs:comment>
    <rdf:type rdf:resource="&dctermsns;SubjectScheme"/>
    <rdfs:isDefinedBy rdf:resource="&dctermsns;"/>
    <rdfs:seeAlso rdf:resource="http://lcweb.loc.gov/catdir/cpso/lcco/lcco.html"/>
  </rdfs:Class>
  <rdfs:Class rdf:about="&dctermsns;DDC">
    <rdfs:label>DDC</rdfs:label>
    <rdfs:comment>Dewey Decimal Classification
  </rdfs:comment>
    <rdf:type rdf:resource="&dctermsns;SubjectScheme"/>
    <rdfs:isDefinedBy rdf:resource="&dctermsns;"/>
    <rdfs:seeAlso rdf:resource="http://www.oclc.org/dewey/index.htm"/>
  </rdfs:Class>
  <rdfs:Class rdf:about="&dctermsns;UDC">
    <rdfs:label>UDC</rdfs:label>
    <rdfs:comment>Universal Decimal Classification
  </rdfs:comment>
    <rdf:type rdf:resource="&dctermsns;SubjectScheme"/>
    <rdfs:isDefinedBy rdf:resource="&dctermsns;"/>
    <rdfs:seeAlso rdf:resource="http://www.udcc.org/"/>
  </rdfs:Class>
  <rdfs:Class rdf:about="&dctermsns;MESH">
    <rdfs:label>MeSH</rdfs:label>
    <rdfs:comment>Medical Subject Headings
  </rdfs:comment>
    <rdf:type rdf:resource="&dctermsns;SubjectScheme"/>
    <rdfs:isDefinedBy rdf:resource="&dctermsns;"/>
    <rdfs:seeAlso rdf:resource="http://www.nlm.nih.gov/mesh/meshhome.html"/>
  </rdfs:Class>
  <!-- End: Subject -->
  <!-- Begin: Description -->
  <!-- Description refinement declarations -->
  <rdf:Property rdf:about="&dctermsns;abstract">
    <rdfs:label>Abstract</rdfs:label>
    <rdfs:comment>A summary of the content of the resource.
  </rdfs:comment>
    <rdfs:subPropertyOf rdf:resource="&dcns;description"/>
    <rdfs:isDefinedBy rdf:resource="&dctermsns;"/>
  </rdf:Property>
  <rdf:Property rdf:about="&dctermsns;tableOfContents">
    <rdfs:label>Table Of Contents</rdfs:label>
    <rdfs:comment>A list of subunits of the content of the resource.
  </rdfs:comment>
    <rdfs:subPropertyOf rdf:resource="&dcns;description"/>
    <rdfs:isDefinedBy rdf:resource="&dctermsns;"/>
  </rdf:Property>
  <rdf:Description rdf:about="&rdfsns;comment">
    <rdfs:subPropertyOf rdf:resource="&dcns;description"/>
  </rdf:Description>
  <!-- End: Description -->
  <!-- Begin: Date -->
  <!-- Date refinement declaration -->
  <rdf:Property rdf:about="&dctermsns;created">
    <rdfs:label>Created</rdfs:label>
    <rdfs:comment>Date of creation of the resource.
  </rdfs:comment>
    <rdfs:subPropertyOf rdf:resource="&dcns;date"/>
    <rdfs:isDefinedBy rdf:resource="&dctermsns;"/>
  </rdf:Property>
  <rdf:Property rdf:about="&dctermsns;issued">
    <rdfs:label>Issued</rdfs:label>
    <rdfs:comment>Date of formal issuance (e.g., publication) of the
    resource.</rdfs:comment>
    <rdfs:subPropertyOf rdf:resource="&dcns;date"/>
    <rdfs:isDefinedBy rdf:resource="&dctermsns;"/>
  </rdf:Property>
  <rdf:Property rdf:about="&dctermsns;modified">
    <rdfs:label>Modified</rdfs:label>
    <rdfs:comment>Date on which the resource was changed.
  </rdfs:comment>
    <rdfs:subPropertyOf rdf:resource="&dcns;date"/>
    <rdfs:isDefinedBy rdf:resource="&dctermsns;"/>
  </rdf:Property>
  <rdf:Property rdf:about="&dctermsns;valid">
    <rdfs:label>Valid</rdfs:label>
    <rdfs:comment>Date (often a range) of validity of a resource.
  </rdfs:comment>
    <rdfs:subPropertyOf rdf:resource="&dcns;date"/>
    <rdfs:isDefinedBy rdf:resource="&dctermsns;"/>
  </rdf:Property>
  <rdf:Property rdf:about="&dctermsns;available">
    <rdfs:label>Available</rdfs:label>
    <rdfs:comment>Date (often a range) that the resource will become or
    did become available.</rdfs:comment>
    <rdfs:subPropertyOf rdf:resource="&dcns;date"/>
    <rdfs:isDefinedBy rdf:resource="&dctermsns;"/>
  </rdf:Property>
  <!-- Encoding Schemes -->
  <rdfs:Class rdf:about="&dctermsns;DateScheme">
    <rdfs:label>Date Encoding Schemes</rdfs:label>
    <rdfs:comment>A set of date encoding schemes and/or formats
  </rdfs:comment>
    <rdfs:isDefinedBy rdf:resource="&dctermsns;"/>
  </rdfs:Class>
  <rdfs:Class rdf:about="&dctermsns;W3CDTF">
    <rdfs:label>W3C-DTF</rdfs:label>
    <rdfs:comment>
   encoded with the W3C Encoding rules for dates and times - a profile based on ISO8601
  </rdfs:comment>
    <rdf:type rdf:resource="&dctermsns;DateScheme"/>
    <rdf:type rdf:resource="&dctermsns;TemporalScheme"/>
    <rdfs:seeAlso rdf:resource="http://www.w3.org/TR/NOTE-datetime"/>
    <rdfs:isDefinedBy rdf:resource="&dctermsns;"/>
  </rdfs:Class>
  <rdfs:Class rdf:about="&dctermsns;Period">
    <rdfs:label>DCMI Period</rdfs:label>
    <rdfs:comment>A specification of the limits of a time interval.
  </rdfs:comment>
    <rdf:type rdf:resource="&dctermsns;DateScheme"/>
    <rdf:type rdf:resource="&dctermsns;TemporalScheme"/>
    <rdfs:seeAlso rdf:resource="http://dublincore.org/documents/dcmi-period/"/>
    <rdfs:isDefinedBy rdf:resource="&dctermsns;"/>
  </rdfs:Class>
  <!-- End: Date -->
  <!-- Begin: format -->
  <!-- format refinement declarations -->
  <rdf:Property rdf:about="&dctermsns;extent">
    <rdfs:label>Extent</rdfs:label>
    <rdfs:comment>The size or duration of the resource.
  </rdfs:comment>
    <rdfs:subPropertyOf rdf:resource="&dcns;format"/>
    <rdfs:isDefinedBy rdf:resource="&dctermsns;"/>
  </rdf:Property>
  <rdf:Property rdf:about="&dctermsns;medium">
    <rdfs:label>Medium</rdfs:label>
    <rdfs:comment>The material or physical carrier of the resource.
  </rdfs:comment>
    <rdfs:subPropertyOf rdf:resource="&dcns;format"/>
    <rdfs:isDefinedBy rdf:resource="&dctermsns;"/>
  </rdf:Property>
  <!-- Encoding Scheme declarations -->
  <rdfs:Class rdf:about="&dctermsns;FormatScheme">
    <rdfs:label>Format Encoding Schemes</rdfs:label>
    <rdfs:comment>A set of format encoding schemes.</rdfs:comment>
    <rdfs:isDefinedBy rdf:resource="&dctermsns;"/>
  </rdfs:Class>
  <rdfs:Class rdf:about="&dctermsns;IMT">
    <rdfs:label>IMT</rdfs:label>
    <rdfs:comment>The Internet media type of the resource.
  </rdfs:comment>
    <rdf:type rdf:resource="&dctermsns;FormatScheme"/>
    <rdfs:isDefinedBy rdf:resource="&dctermsns;"/>
    <rdfs:seeAlso rdf:resource="http://www.isi.edu/in-notes/iana/assignments/media-types/media-types"/>
  </rdfs:Class>
  <!-- End: format -->
  <!-- Begin: Language -->
  <!-- Language refinement declarations -->
  <!-- Encoding Scheme declarations -->
  <rdfs:Class rdf:about="&dctermsns;LanguageScheme">
    <rdfs:label>Language Encoding Schemes</rdfs:label>
    <rdfs:comment>A set of language encoding schemes and/or formats.
  </rdfs:comment>
    <rdfs:isDefinedBy rdf:resource="&dctermsns;"/>
  </rdfs:Class>
  <rdfs:Class rdf:about="&dctermsns;RFC1766">
    <rdfs:label>RFC1766</rdfs:label>
    <rdfs:comment>Internet RFC 1766 'Tags for the identification of
    Language' specifies a two letter code taken from ISO 639, followed
    optionally by a two letter country code taken from ISO 3166.
  </rdfs:comment>
    <rdf:type rdf:resource="&dctermsns;LanguageScheme"/>
    <rdfs:seeAlso rdf:resource="http://www.ietf.org/rfc/rfc1766.txt"/>
    <rdfs:isDefinedBy rdf:resource="&dctermsns;"/>
  </rdfs:Class>
  <rdfs:Class rdf:about="&dctermsns;ISO639-2">
    <rdfs:label>ISO 639-2</rdfs:label>
    <rdfs:comment>ISO 639-2: Codes for the representation of names of
    languages.</rdfs:comment>
    <rdf:type rdf:resource="&dctermsns;LanguageScheme"/>
    <rdfs:seeAlso rdf:resource="http://www.loc.gov/standards/iso639-2/langhome.html"/>
    <rdfs:isDefinedBy rdf:resource="&dctermsns;"/>
  </rdfs:Class>
  <!-- End: language -->
  <!-- Begin: Relation -->
  <!-- Relation refinement declarations -->
  <rdf:Property rdf:about="&dctermsns;isPartOf">
    <rdfs:label>Is Part Of</rdfs:label>
    <rdfs:comment>The described resource is a physical or logical part
    of the referenced resource.</rdfs:comment>
    <rdfs:subPropertyOf rdf:resource="&dcns;relation"/>
    <rdfs:isDefinedBy rdf:resource="&dctermsns;"/>
  </rdf:Property>
  <rdf:Property rdf:about="&dctermsns;hasPart">
    <rdfs:label>Has Part</rdfs:label>
    <rdfs:comment>The described resource includes the referenced resource
    either physically or logically.</rdfs:comment>
    <rdfs:subPropertyOf rdf:resource="&dcns;relation"/>
    <rdfs:isDefinedBy rdf:resource="&dctermsns;"/>
  </rdf:Property>
  <rdf:Property rdf:about="&dctermsns;isVersionOf">
    <rdfs:label>Is Version Of</rdfs:label>
    <rdfs:comment>The described resource is a version, edition, or
    adaptation of the referenced resource. Changes in version imply
    substantive changes in content rather than differences in format.
  </rdfs:comment>
    <rdfs:subPropertyOf rdf:resource="&dcns;relation"/>
    <rdfs:isDefinedBy rdf:resource="&dctermsns;"/>
  </rdf:Property>
  <rdf:Property rdf:about="&dctermsns;hasVersion">
    <rdfs:label>Has Version</rdfs:label>
    <rdfs:comment>The described resource has a version, edition, or
    adaptation, namely, the referenced resource.</rdfs:comment>
    <rdfs:subPropertyOf rdf:resource="&dcns;relation"/>
    <rdfs:isDefinedBy rdf:resource="&dctermsns;"/>
  </rdf:Property>
  <rdf:Property rdf:about="&dctermsns;isFormatOf">
    <rdfs:label>Is Format Of</rdfs:label>
    <rdfs:comment>The described resource is the same intellectual content
    of the referenced resource, but presented in another format.
  </rdfs:comment>
    <rdfs:subPropertyOf rdf:resource="&dcns;relation"/>
    <rdfs:isDefinedBy rdf:resource="&dctermsns;"/>
  </rdf:Property>
  <rdf:Property rdf:about="&dctermsns;hasFormat">
    <rdfs:label>Has Format</rdfs:label>
    <rdfs:comment>The described resource pre-existed the referenced
    resource, which is essentially the same intellectual content presented
    in another format.</rdfs:comment>
    <rdfs:subPropertyOf rdf:resource="&dcns;relation"/>
    <rdfs:isDefinedBy rdf:resource="&dctermsns;"/>
  </rdf:Property>
  <rdf:Property rdf:about="&dctermsns;references">
    <rdfs:label>References</rdfs:label>
    <rdfs:comment>The described resource references, cites, or otherwise
    points to the referenced resource.</rdfs:comment>
    <rdfs:subPropertyOf rdf:resource="&dcns;relation"/>
    <rdfs:isDefinedBy rdf:resource="&dctermsns;"/>
  </rdf:Property>
  <rdf:Property rdf:about="&dctermsns;isReferencedBy">
    <rdfs:label>Is Referenced By</rdfs:label>
    <rdfs:comment>The described resource is referenced, cited, or
    otherwise pointed to by the referenced resource.</rdfs:comment>
    <rdfs:subPropertyOf rdf:resource="&dcns;relation"/>
    <rdfs:isDefinedBy rdf:resource="&dctermsns;"/>
  </rdf:Property>
  <rdf:Property rdf:about="&dctermsns;requires">
    <rdfs:label>Requires</rdfs:label>
    <rdfs:comment>The described resource requires the referenced resource
    to support its function, delivery, or coherence of content.
  </rdfs:comment>
    <rdfs:subPropertyOf rdf:resource="&dcns;relation"/>
    <rdfs:isDefinedBy rdf:resource="&dctermsns;"/>
  </rdf:Property>
  <rdf:Property rdf:about="&dctermsns;isRequiredBy">
    <rdfs:label>Is Required By</rdfs:label>
    <rdfs:comment>The described resource is required by the referenced
    resource, either physically or logically. </rdfs:comment>
    <rdfs:subPropertyOf rdf:resource="&dcns;relation"/>
    <rdfs:isDefinedBy rdf:resource="&dctermsns;"/>
  </rdf:Property>
  <rdf:Property rdf:about="&dctermsns;replaces">
    <rdfs:label>Replaces</rdfs:label>
    <rdfs:comment>The described resource supplants, displaces, or
    supersedes the referenced resource.
  </rdfs:comment>
    <rdfs:subPropertyOf rdf:resource="&dcns;relation"/>
    <rdfs:isDefinedBy rdf:resource="&dctermsns;"/>
  </rdf:Property>
  <rdf:Property rdf:about="&dctermsns;isReplacedBy">
    <rdfs:label>Is Replaced By</rdfs:label>
    <rdfs:comment>The described resource is supplanted, displaced, or
    superseded by the referenced resource.</rdfs:comment>
    <rdfs:subPropertyOf rdf:resource="&dcns;relation"/>
    <rdfs:isDefinedBy rdf:resource="&dctermsns;"/>
  </rdf:Property>
  <rdf:Description rdf:about="&rdfsns;seeAlso">
    <rdfs:subPropertyOf rdf:resource="&dcns;relation"/>
  </rdf:Description>
  <rdf:Description rdf:about="&rdfsns;isDefinedBy">
    <rdfs:subPropertyOf rdf:resource="&dcns;relation"/>
  </rdf:Description>
  <!-- Encoding Scheme declarations -->
  <!-- End: Relation -->
  <!-- Begin: coverage -->
  <!-- Coverage refinement declarations -->
  <rdf:Property rdf:about="&dctermsns;spatial">
    <rdfs:label>Spatial</rdfs:label>
    <rdfs:comment>Spatial characteristics of the intellectual content of
    the resource.</rdfs:comment>
    <rdfs:subPropertyOf rdf:resource="&dcns;coverage"/>
    <rdfs:isDefinedBy rdf:resource="&dctermsns;"/>
  </rdf:Property>
  <rdf:Property rdf:about="&dctermsns;temporal">
    <rdfs:label>Temporal</rdfs:label>
    <rdfs:comment>Temporal characteristics of the intellectual content
    of the resource.</rdfs:comment>
    <rdfs:subPropertyOf rdf:resource="&dcns;coverage"/>
    <rdfs:isDefinedBy rdf:resource="&dctermsns;"/>
  </rdf:Property>
  <!-- Coverage range declarations -->
  <!-- Encoding Schemes -->
  <rdfs:Class rdf:about="&dctermsns;SpatialScheme">
    <rdfs:label>Place Encoding Schemes</rdfs:label>
    <rdfs:comment>A set of geographic place encoding schemes and/or
    formats</rdfs:comment>
    <rdfs:isDefinedBy rdf:resource="&dctermsns;"/>
  </rdfs:Class>
  <rdfs:Class rdf:about="&dctermsns;TGN">
    <rdfs:label>TGN</rdfs:label>
    <rdfs:comment>The Getty Thesaurus of Geographic Names
  </rdfs:comment>
    <rdf:type rdf:resource="&dctermsns;SpatialScheme"/>
    <rdfs:seeAlso rdf:resource="http://www.getty.edu/research/tools/vocabulary/tgn/"/>
    <rdfs:isDefinedBy rdf:resource="&dctermsns;"/>
  </rdfs:Class>
  <rdfs:Class rdf:about="&dctermsns;ISO3166">
    <rdfs:label>ISO3166</rdfs:label>
    <rdfs:comment>ISO3166 Codes for the representation of names of
    countries</rdfs:comment>
    <rdf:type rdf:resource="&dctermsns;SpatialScheme"/>
    <rdfs:seeAlso rdf:resource="http://www.din.de/gremien/nas/nabd/iso3166ma/codlstp1/"/>
    <rdfs:isDefinedBy rdf:resource="&dctermsns;"/>
  </rdfs:Class>
  <rdfs:Class rdf:about="&dctermsns;Box">
    <rdfs:label>DCMI Box</rdfs:label>
    <rdfs:comment>The DCMI Box encoding scheme is a method for identifying
    a region of space using its geographic limits.</rdfs:comment>
    <rdf:type rdf:resource="&dctermsns;SpatialScheme"/>
    <rdfs:seeAlso rdf:resource="http://dublincore.org/documents/dcmi-box/"/>
    <rdfs:isDefinedBy rdf:resource="&dctermsns;"/>
  </rdfs:Class>
  <rdfs:Class rdf:about="&dctermsns;Point">
    <rdfs:label>DCMI Point</rdfs:label>
    <rdfs:comment>DCMI Point is used for identifying a point in space
    using its geographic coordinates</rdfs:comment>
    <rdf:type rdf:resource="&dctermsns;SpatialScheme"/>
    <rdfs:seeAlso rdf:resource="http://dublincore.org/documents/dcmi-point/"/>
    <rdfs:isDefinedBy rdf:resource="&dctermsns;"/>
  </rdfs:Class>
  <rdfs:Class rdf:about="&dctermsns;TemporalScheme">
    <rdfs:label>Encoding Schemes for temporal characteristics
    of the intellectual content of a resource</rdfs:label>
    <rdfs:comment>A set of  encoding schemes and/or
    formats for temporal characteristics of the intellectual
    content of a resource</rdfs:comment>
    <rdfs:isDefinedBy rdf:resource="&dctermsns;"/>
  </rdfs:Class>
  <!-- End: coverage -->
  <!-- Begin: type -->
  <!-- Encoding Schemes -->
  <rdfs:Class rdf:about="&dctermsns;TypeScheme">
    <rdfs:label>Resource Type Encoding Schemes</rdfs:label>
    <rdfs:comment>A set of resource type encoding schemes and/or
    formats</rdfs:comment>
    <rdfs:isDefinedBy rdf:resource="&dctermsns;"/>
  </rdfs:Class>
  <rdfs:Class rdf:about="&dctermsns;DCMIType">
    <rdfs:label>DCMI Type Vocabulary</rdfs:label>
    <rdfs:comment>A list of types used to categorize the nature or
  genre of the content of the resource.</rdfs:comment>
    <rdf:type rdf:resource="&dctermsns;TypeScheme"/>
    <rdfs:seeAlso rdf:resource="http://dublincore.org/documents/dcmi-type-vocabulary/"/>
    <rdfs:seeAlso rdf:resource="&dctypens;"/>
    <rdfs:isDefinedBy rdf:resource="&dctermsns;"/>
  </rdfs:Class>
  <rdf:Description rdf:about="&rdfns;type">
    <rdfs:subPropertyOf rdf:resource="&dcns;type"/>
  </rdf:Description>
  <!-- End: type -->
  <!-- Description of this Schema -->
  <rdf:Description rdf:about="&dctypens;">
    <dc:title>The DCMI Types namespace providing access
   to it's content by means of an RDF Schema</dc:title>
    <dc:publisher>The Dublin Core Metadata Initiative</dc:publisher>
    <dc:description>The Dublin Core Types namespace provides URIs for the
    entries of the DCMI Type Vocabulary. Entries are declared using RDF Schema
    language to support RDF applications.</dc:description>
    <dc:language>English</dc:language>
    <dcterms:requires rdf:resource="http://dublincore.org/documents/dcmi-type-vocabulary/"/>
    <dc:source rdf:resource="http://dublincore.org/documents/dcmi-type-vocabulary/"/>
  </rdf:Description>
  <rdfs:Class rdf:about="&dctermsns;DCMIType">
    <dc:description>
    The DCMI Type Vocabulary provides a general, cross-domain list of approved
    terms that may be used as values for the Resource Type element to identify
    the genre of a resource.
  </dc:description>
    <rdf:type rdf:resource="&dctermsns;TypeScheme"/>
    <rdfs:isDefinedBy rdf:resource="&dctermsns;"/>
  </rdfs:Class>
  <rdfs:Class rdf:about="&dctypens;Collection">
    <rdfs:label>Collection</rdfs:label>
    <rdfs:isDefinedBy rdf:resource="&dctypens;"/>
    <rdfs:seeAlso rdf:resource="http://dublincore.org/documents/dcmi-type-vocabulary/"/>
    <rdfs:comment>
    A collection is an aggregation of items. The term collection means that
    the resource is described as a group; its parts may be separately
    described and navigated.
  </rdfs:comment>
    <rdf:type rdf:resource="&dctermsns;DCMIType"/>
  </rdfs:Class>
  <rdfs:Class rdf:about="&dctypens;Dataset">
    <rdfs:label>Dataset</rdfs:label>
    <rdfs:isDefinedBy rdf:resource="&dctypens;"/>
    <rdfs:seeAlso rdf:resource="http://dublincore.org/documents/dcmi-type-vocabulary/"/>
    <rdfs:comment>
    A dataset is information encoded in a defined structure (for example,
    lists, tables, and databases), intended to be useful for direct
    machine processing.
  </rdfs:comment>
    <rdf:type rdf:resource="&dctermsns;DCMIType"/>
  </rdfs:Class>
  <rdfs:Class rdf:about="&dctypens;Event">
    <rdfs:label>Event</rdfs:label>
    <rdfs:isDefinedBy rdf:resource="&dctypens;"/>
    <rdfs:seeAlso rdf:resource="http://dublincore.org/documents/dcmi-type-vocabulary/"/>
    <rdfs:comment>
    An event is a non-persistent, time-based occurrence. Metadata for an
    event provides descriptive information that is the basis for discovery
    of the purpose, location, duration, responsible agents, and links to
    related events and resources. The resource of type event may not be
    retrievable if the described instantiation has expired or is yet to occur.
    Examples - exhibition, web-cast, conference, workshop, open-day,
    performance, battle, trial, wedding, tea-party, conflagration.
  </rdfs:comment>
    <rdf:type rdf:resource="&dctermsns;DCMIType"/>
  </rdfs:Class>
  <rdfs:Class rdf:about="&dctypens;Image">
    <rdfs:label>Image</rdfs:label>
    <rdfs:isDefinedBy rdf:resource="&dctypens;"/>
    <rdfs:seeAlso rdf:resource="http://dublincore.org/documents/dcmi-type-vocabulary/"/>
    <rdfs:comment>
    An image is a primarily symbolic visual representation other than text.
    For example - images and photographs of physical objects, paintings,
    prints, drawings, other images and graphics, animations and moving
    pictures, film, diagrams, maps, musical notation. Note that image may
    include both electronic and physical representations.
  </rdfs:comment>
    <rdf:type rdf:resource="&dctermsns;DCMIType"/>
  </rdfs:Class>
  <rdfs:Class rdf:about="&dctypens;InteractiveResource">
    <rdfs:label>Interactive Resource</rdfs:label>
    <rdfs:isDefinedBy rdf:resource="&dctypens;"/>
    <rdfs:seeAlso rdf:resource="http://dublincore.org/documents/dcmi-type-vocabulary/"/>
    <rdfs:comment>
    An interactive resource is a resource which requires interaction from the
    user to be understood, executed, or experienced. For example - forms on web
    pages, applets, multimedia learning objects, chat services, virtual reality.
  </rdfs:comment>
    <rdf:type rdf:resource="&dctermsns;DCMIType"/>
  </rdfs:Class>
  <rdfs:Class rdf:about="&dctypens;Software">
    <rdfs:label>Software</rdfs:label>
    <rdfs:isDefinedBy rdf:resource="&dctypens;"/>
    <rdfs:seeAlso rdf:resource="http://dublincore.org/documents/dcmi-type-vocabulary/"/>
    <rdfs:comment>
    Software is a computer program in source or compiled form which may be
    available for installation non-transiently on another machine. For
    software which exists only to create an interactive environment, use
    interactive instead.
  </rdfs:comment>
    <rdf:type rdf:resource="&dctermsns;DCMIType"/>
  </rdfs:Class>
  <rdfs:Class rdf:about="&dctypens;Service">
    <rdfs:label>Service</rdfs:label>
    <rdfs:isDefinedBy rdf:resource="&dctypens;"/>
    <rdfs:seeAlso rdf:resource="http://dublincore.org/documents/dcmi-type-vocabulary/"/>
    <rdfs:comment>
    A service is a system that provides one or more functions of value to the
    end-user. Examples include: a photocopying service, a banking service,
    an authentication service, interlibrary loans, a Z39.50 or Web server.
  </rdfs:comment>
    <rdf:type rdf:resource="&dctermsns;DCMIType"/>
  </rdfs:Class>
  <rdfs:Class rdf:about="&dctypens;Sound">
    <rdfs:label>Sound</rdfs:label>
    <rdfs:isDefinedBy rdf:resource="&dctypens;"/>
    <rdfs:seeAlso rdf:resource="http://dublincore.org/documents/dcmi-type-vocabulary/"/>
    <rdfs:comment>
    A sound is a resource whose content is primarily intended to be rendered
    as audio. For example - a music playback file format, an audio compact
    disc, and recorded speech or sounds.
  </rdfs:comment>
    <rdf:type rdf:resource="&dctermsns;DCMIType"/>
  </rdfs:Class>
  <rdfs:Class rdf:about="&dctypens;Text">
    <rdfs:label>Text</rdfs:label>
    <rdfs:isDefinedBy rdf:resource="&dctypens;"/>
    <rdfs:seeAlso rdf:resource="http://dublincore.org/documents/dcmi-type-vocabulary/"/>
    <rdfs:comment>
    A text is a resource whose content is primarily words for reading.
    For example - books, letters, dissertations, poems, newspapers, articles,
    archives of mailing lists. Note that facsimiles or images of texts are still
    of the genre text.
  </rdfs:comment>
    <rdf:type rdf:resource="&dctermsns;DCMIType"/>
  </rdfs:Class>
</rdf:RDF>
